LeanCats/Data.lean
@@ -1,0 +1,32 @@
+inductive Thread : Type where
+  | mk: Nat -> Thread
+deriving BEq, Repr, DecidableEq
+
+abbrev write := "write"
+abbrev read := "read"
+
+/-
+Actions are of several kinds, which we detail in the course of this article. For now, we
+only consider read and write events relative to memory locations. For example, for the
+location x, we can have a read of the value 0 noted Rx = 0, or a write of the value 1,
+noted Wx = 1. We write proc(e) for the thread holding the event e and addr(e) for its
+address, or memory location.
+-/
+structure Action : Type where
+  action : String
+  target : String
+  -- For read, the value can not be determined at the begining.
+  value : Option Nat
+  isFirstWrite : Bool
+  isFinalWrite : Bool
+deriving BEq, Repr, DecidableEq
+
+/-
+-/
+structure Event where
+  (id : String)   -- Unique identifier
+  (t_id : Nat)      -- Thread ID
+  (t : Thread)    -- Associated thread
+  (ln : Nat)        -- Line number or position
+  (a : Action) -- Action performed
+deriving BEq, Repr, DecidableEq
