LeanCats/Lemmas.lean
@@ -1,0 +1,177 @@
+import LeanCats.HerdingCats
+
+open Primitives
+
+lemma tc_step_N_swap
+  (n : Nat)
+  (tc : List (Event × Event)) :
+  tc_step_N n (tc_step tc) = tc_step (tc_step_N n tc) :=
+  by
+    induction n generalizing tc with
+    | zero => {
+      simp
+    }
+    | succ n' h' => {
+      rw [tc_step_N]
+      rw [tc_step_N]
+      rw [h' (tc_step tc)]
+    }
+
+lemma tc_step_N_add (m n : Nat) (tc : List (Event × Event)) :
+  tc_step_N (m + n) tc = tc_step_N n (tc_step_N m tc) := by
+  induction m generalizing n with
+  | zero =>
+    simp [tc_step_N]
+  | succ m' ih =>
+    repeat rw [tc_step_N]
+    have h : tc_step_N (m' + n + 1) tc = tc_step_N (n + 1) (tc_step_N m' tc) :=
+      by
+        apply ih (n + 1)
+    nth_rewrite 2 [tc_step_N] at h
+    rw [Nat.add_assoc]
+    nth_rewrite 2 [Nat.add_comm]
+    rw [<-Nat.add_assoc]
+    rw [h]
+    nth_rewrite 2 [tc_step_N_swap]
+    rfl
+
+  lemma tc_base_is_tc
+  {a b : Event}
+  (r : Event -> Event -> Prop)
+  (elems : List Event)
+  [DecidableRel r]
+  : (a, b) ∈ tc_base r elems -> Relation.TransGen r a b :=
+  by
+    intro h
+    simp_all
+    have rab : r a b :=
+      by
+        aesop
+    apply Relation.TransGen.single
+    exact rab
+
+lemma tc_step_contains_prev_step
+  {a b : Event}
+  (tc : List (Event × Event))
+  : (a, b) ∈ tc_step tc -> (a, b) ∈ tc_step (tc_step tc) :=
+  by
+    aesop
+
+lemma tc_step_contains_input
+  (tc : List (Event × Event))
+  : tc ⊆ tc_step tc :=
+  by
+    simp
+
+lemma tc_step_base_is_tc
+  {a b : Event}
+  {r : Event -> Event -> Prop}
+  [DecidableRel r]
+  (input : List Event)
+  : (a, b) ∈ tc_step (tc_base r input) -> Relation.TransGen r a b :=
+  by
+    intro hstep
+    simp at hstep
+    aesop
+    {
+      apply Relation.TransGen.single
+      exact right
+    }
+    {
+      apply Relation.TransGen.single
+      exact right
+    }
+
+lemma tc_step_contains_prev
+  {a b : Event}
+  (tc : List (Event × Event))
+  : (a, b) ∈ tc_step tc -> (a, b) ∈ tc :=
+  by
+    aesop
+
+lemma tc_N_succ_steps_includes_N_succ
+  (n : Nat)
+  (tc : List (Event × Event))
+  : tc_step_N n tc ⊆ tc_step_N (n+1) tc :=
+    by
+      intro h
+      induction n with
+      | zero => {
+        aesop
+      }
+      | succ n' h' => {
+        intro h''
+        unfold tc_step_N
+        unfold tc_step_N
+        rw [tc_step_N_swap]
+        rw [tc_step_N_swap]
+        apply tc_step_contains_prev_step
+        unfold tc_step_N at h''
+        rw [tc_step_N_swap] at h''
+        exact h''
+      }
+
+lemma tc_N_steps_in_tc_N_succ
+  {a b : Event}
+  (n : Nat)
+  (tc : List (Event × Event))
+  : (a, b) ∈ tc_step_N (n+1) tc -> (a, b) ∈ tc_step_N (n) tc :=
+    by
+      intro h
+      induction n generalizing tc with
+      | zero => {
+        aesop
+      }
+      | succ n' h' => {
+        apply (h' (tc_step tc)) h
+      }
+
+lemma tc_N_steps_in_tc_N_succ'
+  {a b : Event}
+  (n : Nat)
+  (r : Event -> Event -> Prop)
+  [DecidableRel r]
+  (input : List Event)
+  : (a, b) ∈ tc_step_N (n+1) (tc_base r input) -> (a, b) ∈ tc_step_N (n) (tc_base r input) :=
+    by
+      intro h
+      apply tc_N_steps_in_tc_N_succ
+      aesop
+
+lemma tc_N_steps_is_tc
+  {a b : Event}
+  (n : Nat)
+  (r : Event -> Event -> Prop)
+  [DecidableRel r]
+  (input : List Event)
+  : (a, b) ∈ tc_step_N n (tc_base r input) -> Relation.TransGen r a b := by
+    intro h'
+    induction n with
+    | zero => {
+      simp at h'
+      have hrab : r a b :=
+        by
+          aesop
+      apply Relation.TransGen.single
+      exact hrab
+    }
+    | succ n' h'' => {
+      apply h''
+      apply tc_N_steps_in_tc_N_succ'
+      exact h'
+    }
+
+lemma comp_tc_towards_tc
+  {a b : Event}
+  (r : Event -> Event -> Prop)
+  [DecidableRel r]
+  (input : List Event) :
+  a ∈ input
+  -> b ∈ input
+  -> (a, b) ∈ comp_tc input r
+  -> Relation.TransGen r a b := by
+    intro ha hb
+    unfold comp_tc
+    intro h
+    apply tc_N_steps_is_tc
+    apply h
